DiscreteStream.v
@@ -1,0 +1,327 @@
+Require Import Coq.Classes.RelationClasses.
+Require Import Coq.Classes.Morphisms.
+Require Coq.Lists.List.
+
+Set Implicit Arguments.
+Set Strict Implict.
+
+Section with_state.
+
+  Variable ST : Type.
+  Variable ST_eq : ST -> ST -> Prop.
+
+  (* A trace is an infinite stream of states.
+   *)
+  CoInductive stream : Type :=
+  | Continue : ST -> stream -> stream.
+
+  Notation "a ':::' ts" := (Continue a ts) (at level 70, right associativity).
+  Definition hd (tr : stream) : ST :=
+    match tr with
+    | Continue hd _ => hd
+    end.
+
+  Definition tl (tr : stream) : stream :=
+    match tr with
+    | Continue _ tl => tl
+    end.
+
+  CoInductive stream_eq : stream -> stream -> Prop :=
+  | Discr_eq : forall a b,
+      ST_eq (hd a) (hd b) ->
+      stream_eq (tl a) (tl b) ->
+      stream_eq a b.
+
+  Global Instance Proper_hd : Proper (stream_eq ==> ST_eq) hd.
+  Proof. do 2 red; destruct 1; auto. Qed.
+
+  Global Instance Proper_tl : Proper (stream_eq ==> stream_eq) tl.
+  Proof. do 2 red; destruct 1; auto. Qed.
+
+  Global Instance Reflexive_stream_eq {Refl_r : Reflexive ST_eq} : Reflexive stream_eq.
+  Proof.
+    red. cofix Reflexive_stream_eq.
+    constructor. reflexivity. eapply Reflexive_stream_eq.
+  Qed.
+
+  Global Instance Symmetric_stream_eq {Sym_r : Symmetric ST_eq} : Symmetric stream_eq.
+  Proof.
+    red. cofix Symmetric_stream_eq.
+    constructor.
+    { destruct H. symmetry. eassumption. }
+    { destruct H. eapply Symmetric_stream_eq. eassumption. }
+  Qed.
+
+  Global Instance Transitive_stream_eq {Trans_r : Transitive ST_eq} : Transitive stream_eq.
+  Proof.
+    red. cofix Transitive_stream_eq.
+    constructor.
+    { destruct H; destruct H0; etransitivity; eauto. }
+    { destruct H; destruct H0. eapply Transitive_stream_eq; eauto. }
+  Qed.
+
+  Global Instance PreOrder_stream_eq (PO : PreOrder ST_eq)
+  : PreOrder stream_eq.
+  Proof.
+    destruct PO.
+    constructor.
+    { eapply Reflexive_stream_eq. }
+    { eapply Transitive_stream_eq. }
+  Qed.
+
+End with_state.
+
+Section skips_to.
+  Context {T : Type}.
+
+  Inductive skips_to (s : stream T) : stream T -> Prop :=
+  | Now : forall t, stream_eq eq s t -> skips_to s t
+  | Later : forall t, skips_to s (tl t) -> skips_to s t.
+
+  Lemma skips_to_next
+  : forall s s',
+      skips_to s s' ->
+      skips_to (tl s) s'.
+  Proof.
+    induction 1.
+    { apply Later. apply Now. eapply Proper_tl. assumption. }
+    { apply Later. assumption. }
+  Qed.
+
+  Global Instance Proper_skips_to_impl
+  : Proper (stream_eq eq ==> stream_eq eq ==> Basics.impl) skips_to.
+  Proof.
+    do 4 red.
+    intros.
+    generalize dependent y. generalize dependent y0.
+    induction H1; intros.
+    { eapply Now.
+      etransitivity; try eassumption.
+      etransitivity; try eassumption.
+      symmetry; eauto. }
+    { eapply Later.
+      eapply IHskips_to; eauto.
+      destruct H0; auto. }
+  Qed.
+
+  Global Instance Proper_skips_to_iff
+  : Proper (stream_eq eq ==> stream_eq eq ==> iff) skips_to.
+  Proof.
+    do 4 red. split.
+    - rewrite H. rewrite H0. tauto.
+    - rewrite H. rewrite H0. tauto.
+  Qed.
+
+  Global Instance Transitive_skips_to : Transitive skips_to.
+  Proof.
+    red.
+    intros x y z H.
+    induction H using skips_to_ind; eauto using skips_to_next.
+    rewrite H. auto.
+  Qed.
+
+  Global Instance Reflexive_skips_to : Reflexive skips_to.
+  Proof.
+    red. intros. eapply Now. reflexivity.
+  Qed.
+End skips_to.
+
+(* Functorial *)
+Require Import ExtLib.Structures.Functor.
+Require Import ExtLib.Structures.Applicative.
+
+Section functorial.
+  Context {state1 state2 : Type}.
+  Variable morphism : state1 -> state2.
+
+  CoFixpoint fmap_stream (tr : @stream state1)
+  : @stream state2 :=
+    match tr with
+    | Continue s c => Continue (morphism s) (fmap_stream c)
+    end.
+End functorial.
+
+Theorem fmap_continue_compose : forall A B C (f : B -> C) (g : A -> B) (tr : stream _),
+    stream_eq eq(fmap_stream f (fmap_stream g tr)) (fmap_stream (fun x => f (g x)) tr).
+Proof.
+  intros A B C f g.
+  cofix cih.
+  intros.
+  constructor.
+  - destruct tr; reflexivity.
+  - destruct tr. simpl. eapply cih.
+Qed.
+
+Instance Functor_stream : Functor stream :=
+{ fmap := @fmap_stream }.
+
+CoFixpoint forever {T} (v : T) : stream T :=
+  Continue v (forever v).
+
+CoFixpoint stream_ap {T U : Type} (f : stream (T -> U)) (x : stream T) : stream U :=
+  Continue ((hd f) (hd x)) (stream_ap (tl f) (tl x)).
+
+Instance Applicative_stream : Applicative stream :=
+{ pure := @forever
+; ap := @stream_ap
+}.
+
+Definition stream_zip {T U V : Type} (f : T -> U -> V) (a : stream T) (b : stream U) : stream V :=
+  ap (ap (pure f) a) b.
+
+Arguments skips_to {ST} _ _ : rename.
+Arguments hd {ST} _.
+Arguments tl {ST} _.
+Arguments Transitive_skips_to {ST} _ _ _ _ _ : rename.
+Arguments Reflexive_skips_to {ST} _ : rename.
+
+Section extra_stream_properties.
+  Context {T U V : Type} (Rt : T -> T -> Prop) (Ru : U -> U -> Prop) (Rv : V -> V -> Prop).
+
+  CoFixpoint prefixes {T} (acc : list T) (tr : stream T) : stream (list T) :=
+    match tr with
+    | Continue t tr => Continue acc (prefixes (t :: acc) tr)
+    end.
+
+  Lemma stream_zip_snd : forall {T U} (a : stream T) (b : stream U),
+      stream_eq eq (stream_zip (fun _ x => x) a b) b.
+  Proof using.
+    do 2 intro.
+    cofix stream_zip_snd.
+    destruct a; destruct b.
+    constructor.
+    - reflexivity.
+    - simpl.  simpl. eapply stream_zip_snd.
+  Qed.
+
+  Lemma stream_zip_fst : forall {T U} (a : stream T) (b : stream U),
+      stream_eq eq (stream_zip (fun x _ => x) a b) a.
+  Proof using.
+    do 2 intro.
+    cofix stream_zip_fst.
+    destruct a; destruct b.
+    constructor.
+    - reflexivity.
+    - simpl.  simpl. eapply stream_zip_fst.
+  Qed.
+
+  Lemma stream_eq_equiv : forall (a b c d : stream T),
+      stream_eq Rt b c ->
+      stream_eq eq a b ->
+      stream_eq eq c d ->
+      stream_eq Rt a d.
+  Proof.
+    cofix stream_eq_equiv.
+    intros.
+    destruct H; destruct H0; destruct H1.
+    constructor.
+    { rewrite H0. rewrite <- H1. assumption. }
+    { eapply stream_eq_equiv; eassumption. }
+  Qed.
+
+  Global Instance Proper_stream_eq : Proper (stream_eq eq ==> stream_eq eq ==> iff) (stream_eq Rt).
+  Proof.
+    do 3 red. split; intros.
+    - eapply stream_eq_equiv; eauto. symmetry; eauto.
+    - eapply stream_eq_equiv; eauto. symmetry; eauto.
+  Qed.
+
+  Lemma fmap_stream_eq : forall f g,
+      (Rt ==> Ru)%signature f g ->
+      forall (a d : stream U) (b c : stream T),
+        stream_eq Rt b c ->
+        stream_eq eq a (fmap f b) ->
+        stream_eq eq (fmap g c) d ->
+        stream_eq Ru a d.
+  Proof.
+    intros f g Hf.
+    cofix fmap_stream_eq.
+    intros.
+    inversion H; inversion H0; inversion H1; subst.
+    constructor.
+    { simpl. eapply Hf in H2. rewrite H6. rewrite <- H10.
+      clear - H2.
+      destruct b; destruct c. eapply H2. }
+    { eapply (@fmap_stream_eq _ _ _ _ H3).
+      - etransitivity; [ eassumption | clear ].
+        constructor; destruct b; reflexivity.
+      - etransitivity; [ clear | eassumption ].
+        constructor; destruct c; reflexivity. }
+  Qed.
+
+  Global Instance Proper_fmap_stream_eq :
+    Proper ((Rt ==> Ru) ==> stream_eq Rt ==> stream_eq Ru) fmap.
+  Proof.
+    do 3 red. intros.
+    eapply fmap_stream_eq; solve [ eassumption | reflexivity ].
+  Qed.
+
+  Lemma stream_eq_stream_zip (f g : T -> U -> V) :
+    (Rt ==> Ru ==> Rv)%signature f g ->
+    forall a b c d X Y,
+      stream_eq Rt a b ->
+      stream_eq Ru c d ->
+      stream_eq eq X (stream_zip f a c) ->
+      stream_eq eq (stream_zip g b d) Y ->
+      stream_eq Rv X Y.
+  Proof.
+    intro Hfg.
+    cofix stream_eq_stream_zip.
+    do 4 inversion 1; subst.
+    constructor.
+    { rewrite H10. rewrite <- H15.
+      destruct c; destruct d; simpl in *. eapply Hfg; eassumption. }
+    { eapply (@stream_eq_stream_zip _ _ _ _ _ _ H1 H6).
+      - etransitivity; [ eassumption | clear ].
+        destruct a; destruct c; constructor; try reflexivity.
+      - etransitivity; [ clear | eassumption ].
+        destruct a; destruct c; constructor; try reflexivity. }
+  Qed.
+
+  Global Instance Proper_stream_zip :
+    Proper ((Rt ==> Ru ==> Rv) ==> stream_eq Rt ==> stream_eq Ru ==> stream_eq Rv) stream_zip.
+  Proof.
+    do 4 red. intros.
+    eapply stream_eq_stream_zip; solve [ eassumption | reflexivity ].
+  Qed.
+
+  Lemma fmap_stream_stream_zip_compose' {W} (Rw : W -> W -> Prop) (f f' : T -> U -> V) (g g' : V -> W) :
+    (Rt ==> Ru ==> Rv)%signature f f' ->
+    (Rv ==> Rw)%signature g g' ->
+    forall a b c d X Y,
+      stream_eq Rt a b ->
+      stream_eq Ru c d ->
+      stream_eq eq X (fmap_stream g (stream_zip f a c)) ->
+      stream_eq eq (stream_zip (fun a b => g' (f' a b)) b d) Y ->
+      stream_eq Rw X Y.
+  Proof.
+    intros Hf Hg.
+    cofix fmap_stream_stream_zip_compose'.
+    do 4 inversion 1; subst.
+    constructor.
+    { rewrite H10. rewrite <- H15.
+      destruct a; destruct b; destruct c; destruct d; simpl in *.
+      eapply Hg. eapply Hf; eauto. }
+    { eapply fmap_stream_stream_zip_compose'; try eassumption. }
+  Qed.
+
+  Global Instance Proper_Continue : Proper (Rt ==> stream_eq Rt ==> stream_eq Rt) (@Continue T).
+  Proof.
+    compute; intros.
+    constructor; eauto.
+  Qed.
+
+  Theorem stream_eq_eta (x : stream T) : stream_eq eq x (Continue (hd x) (tl x)).
+  Proof.
+    constructor; reflexivity.
+  Qed.
+
+End extra_stream_properties.
+
+Theorem fmap_stream_stream_zip_compose {T U V W} (f : T -> U -> V) (g : V -> W) :
+  forall a b,
+    stream_eq eq (fmap_stream g (stream_zip f a b)) (stream_zip (fun a b => g (f a b)) a b).
+Proof.
+  intros. eapply fmap_stream_stream_zip_compose' with (Rt := eq) (Ru := eq) (Rv :=eq);
+          try solve [ eassumption | reflexivity ].
+Qed.
