LTS.v
@@ -1,0 +1,167 @@
+From Coq Require Import
+     Relations
+     List
+     Lia.
+
+Import ListNotations.
+From RDS Require Import
+     Relations
+     DiscreteStream.
+
+From ExtLib Require Import
+     Structures.Monad
+     Core.RelDec
+     Structures.Maps
+     Data.Map.FMapAList.
+
+Section ETL.
+
+  Variables (uid: Set) (atom: Set) (heap: Set).
+
+  Inductive fact : Set :=
+  | Ret: atom -> fact
+  | Knows: uid -> fact -> fact.
+  
+  (* Toy programming language executed by agents *)
+  Inductive prog :=
+  | Comp: prog
+  | Send: uid -> fact -> prog
+  | Recv: prog.
+
+  Definition db := list fact.
+  Definition trace := stream (uid * heap * prog * db)%type.
+
+  Variable init_trace: uid -> trace -> Prop.
+
+  Parameter eqdec_uid: RelDec (@eq uid).  
+  Global Existing Instance eqdec_uid.
+
+  Parameter eqdec_atom: RelDec (@eq atom).  
+  Global Existing Instance eqdec_atom.
+
+  Global Instance eqdec_msg: RelDec (@eq fact) := {
+      rel_dec := fix rec(a b: fact) :=
+        match a,b with
+        | Ret a, Ret b => rel_dec a b
+        | Knows ua fa, Knows ub fb =>
+            andb (rel_dec ua ub) (rec fa fb)
+        | _, _ => false
+        end
+    }.
+
+  Variable (transition: uid -> relation (heap*prog)).  
+  Variable (transition_determ: forall u s s' s'',
+               transition u s s' ->
+               transition u s s'' -> s' = s'').
+
+  (* Execute program Comp and produce new program p' and new heap st' *)
+  Reserved Notation "a '-->' b" (at level 89).
+  Inductive cstep: uid * heap * prog * db -> uid * heap * prog * db -> Prop :=
+  | DoComp: forall st st' p' (d: db) (agent: uid),
+      transition agent (st, Comp) (st', p') ->
+      cstep (agent, st, Comp, d) (agent, st', p', d)
+  where "a '-->' b" := (cstep a b).
+
+  (** A distributed system is a list of traces *)
+  Definition system := list trace.
+  
+  Reserved Notation "a '==>' b" (at level 90).
+  
+  Inductive step: system -> system  -> Prop :=
+  | LocalStep: forall a a' past hds tls,
+    a --> a' ->
+    hds ++ [ Continue a past ] ++ tls ==>
+    hds ++ [ Continue a' (Continue a past) ] ++ tls
+  | MsgDeliver: forall hds mid tls ua ub ha hb ha' hb' dba dbb m pa pb past past',
+      transition ua (ha, Send ub m) (ha', pa) ->
+      transition ub (hb, Recv) (hb', pb) ->
+      hds
+      ++ [ Continue  (ua, ha, Send ub m, dba) past ]
+      ++ mid
+      ++ [ Continue (ub, hb, Recv, dbb) past' ]
+      ++ tls ==>
+      hds
+      ++ [ Continue (ua, ha, pa, dba)
+             (Continue (ua, ha', Send ub m, dba) past) ]
+      ++ mid
+      ++ [ Continue (ub, hb', pb, (Knows ua m) :: dbb)
+             (Continue (ub, hb, Recv, dbb) past') ]
+      ++ tls
+  where "a '==>' b" := (step a b).
+
+  Notation "a '==>*' b" := (step ^* a b) (at level 40).
+
+  Notation traceProp := (trace -> Prop).
+  Notation stateProp := (uid * heap * prog * db -> Prop).
+
+  Definition and (P Q : traceProp) : traceProp :=
+    fun str => P str /\ Q str.
+
+  Definition and_state (P Q : stateProp) : stateProp :=
+    fun s => P s /\ Q s.
+
+  Definition or (P Q : traceProp) : traceProp :=
+    fun str => P str \/ Q str.
+
+  Definition or_state (P Q : stateProp) : stateProp :=
+    fun s => P s \/ Q s.
+
+  (** How to compose 'implies' and '==>*' *)
+  Definition leads_to_state (P Q : stateProp) : Prop :=
+    forall s t , P s -> s --> t -> Q t.
+
+  (****************************** Temporal basic operators *************************)
+  Definition next (P : traceProp) : traceProp :=
+    fun str => P (tl str).
+
+  CoInductive always (P : traceProp) : traceProp :=
+    C_always :
+      forall s0 (str : trace),
+      P (Continue s0 str) -> always P str -> always P (Continue s0 str).
+  
+  Inductive eventually (P : traceProp) : traceProp :=
+  | ev_h : forall str : trace, P str -> eventually P str
+  | ev_t :
+    forall s (str : trace),
+      eventually P str -> eventually P (Continue s str).
+  
+  Inductive until (P Q : traceProp) : traceProp :=
+  | until_h : forall str : trace, Q str -> until P Q str
+  | until_t :
+    forall s (str : trace),
+      P (Continue s str) -> until P Q str -> until P Q (Continue s str).
+  
+  CoInductive unless (P Q : traceProp) : traceProp :=
+  | unless_h : forall str : trace, Q str -> unless P Q str
+  | unless_t :
+    forall s (str : trace),
+      P (Continue s str) -> unless P Q str -> unless P Q (Continue s str).
+
+
+(****************************** Temporal derived operators ***********************)
+
+Definition infinitely_often (P : traceProp) : 
+  traceProp := always (eventually P).
+
+Definition implies (P Q : traceProp) : traceProp :=
+  always (fun str : trace => P str -> Q str).
+
+Definition is_followed (P Q : traceProp) (str : trace) : Prop :=
+  P str -> eventually Q str.
+
+Definition is_always_followed (P Q : traceProp) : 
+  traceProp := always (is_followed P Q).
+
+Definition eventually_permanently (P : traceProp) : 
+  traceProp := eventually (always P).
+
+Definition once_always (P Q : traceProp) : traceProp :=
+  implies P (always Q).
+
+Definition leads_to_via (P Q R : traceProp) : 
+  traceProp := implies P (until Q R).
+
+Definition once_until (P Q : traceProp) : traceProp :=
+  leads_to_via P P Q.
+
+End ETL.
